To be continued.

sparkfrontend/spark2cmproofs.v
@@ -950,7 +950,7 @@ Definition stbl_var_types_ok st :=
 
 (** The Memory bisimilarity/invariant property states that
 
- - Spark stack [s] is ok wrt overflows
+ -[me_overflow] Spark stack [s] is ok wrt overflows 
  - Compilation environment [CE] contains exactly variables of spark
    stack [s]
  - All variable of [CE] are non overlapping (spark property)
@@ -1177,6 +1177,11 @@ Proof.
       unfold Values.Val.of_bool.
       reflexivity.
 Qed.
+
+  
+
+  
+
 
 
 (** Hypothesis renaming stuff *)
@@ -2436,17 +2441,124 @@ Qed.
 
 Ltac rename_transl_exprlist h th :=
   match th with
-  | transl_exprlist _ _ ?x = Error _ => fresh "h_incr_order_fr_Err_" x
-  | transl_exprlist _ _ _ = Error _ => fresh "h_incr_order_fr_Err"
-  | transl_exprlist _ _ ?x = Some ?y => fresh "h_incr_order_fr_" x "_" y
-  | transl_exprlist _ _ ?x = Some _ => fresh "h_incr_order_fr_" x
-  | transl_exprlist _ _ _ = _ => fresh "h_incr_order_fr"
+  | transl_exprlist _ _ ?x = Error _ => fresh "h_trans_exprl_Err_" x
+  | transl_exprlist _ _ _ = Error _ => fresh "h_trans_exprl_Err"
+  | transl_exprlist _ _ ?x = Some ?y => fresh "h_trans_exprl_" x "_" y
+  | transl_exprlist _ _ ?x = Some _ => fresh "h_trans_exprl_" x
+  | transl_exprlist _ _ _ = _ => fresh "h_trans_exprl"
+
+  | transl_paramexprlist _ _ ?x _ = Error _ => fresh "h_trans_prmexprl_Err_" x
+  | transl_paramexprlist _ _ _ _ = Error _ => fresh "h_trans_prmexprl_Err"
+  | transl_paramexprlist _ _ ?x _ = Some ?y => fresh "h_trans_prmexprl_" x "_" y
+  | transl_paramexprlist _ _ ?x _ = Some _ => fresh "h_trans_prmexprl_" x
+  | transl_paramexprlist _ _ _ _ = _ => fresh "h_trans_prmexprl"
+
+  | eval_exprlist _ _ _ _ ?x Error _ => fresh "h_eval_exprlist_Err_" x
+  | eval_exprlist _ _ _ _ _ Error _ => fresh "h_eval_exprlist_Err"
+  | eval_exprlist _ _ _ _ ?x (Some ?y) => fresh "h_eval_exprlist_" x "_" y
+  | eval_exprlist _ _ _ _ ?x (Some _) => fresh "h_eval_exprlist_" x
+  | eval_exprlist _ _ _ _ _ _ => fresh "h_eval_exprlist"
   | _ => rename_hyp_incro h th
   end.
 Ltac rename_hyp ::= rename_transl_exprlist.
 
-Opaque transl_expr.
 
+(* Property linking spark args expr list , spark args value
+           list , Cminor args expr list and Cminor args value list. We
+           need to talk a bout expressions because Out and InOut
+           parameters are translated into names (and not expressions)
+           in order to be able to have there cminor address. Once the
+           prelude of the function is executed, all variables are in
+           the stack as standard variables. *)
+
+Section is_copy.
+  Variables (stbl : symboltable) (CE : compilenv)   (g : genv) (sp : Values.val) (locenv : env) (m : mem) (s : stack).
+
+  (* FIXME: copy_in ne doit pas prendre une liste de value, mais les calculer à
+     la volée, car on ne peut pas faire autrement pour spécifier le Out. *)
+  (** [is_copy_in le lprms lv_t] means that in the current environment, lev_t
+      correspond to the values that should be stored in the local variables
+      of a function having lprm as parameter list. That is: the value of the
+      argument when In, its address otherwise (with the correct value at the
+      address when In_Out).  *)
+  Inductive is_copy_in: list expression -> list parameter_specification -> list Values.val -> Prop :=
+  | Is_copy_in_nil: is_copy_in nil nil nil
+  | Is_copy_in_In: ∀ e le prm lprm v v_t lv_t,
+      parameter_mode prm = In ->
+      eval_expr stbl s e (Normal v) ->
+      transl_value v v_t ->
+      is_copy_in  le lprm lv_t ->
+      is_copy_in (e::le) (prm::lprm) (v_t::lv_t)
+  | Is_copy_in_In_Out: ∀ astnum le prm lprm nme v addr_t v_t nme_t lv_t,
+      parameter_mode prm = In_Out ->
+      transl_name stbl CE nme = OK nme_t -> (* nme_t is the expresion denoting the address where nme is stored in Cminor *)
+      eval_expr stbl s (E_Name astnum nme) (Normal v) -> (* addr is the evaluated variable in spark *)
+      Cminor.eval_expr g sp locenv m nme_t addr_t  -> (* v_t is the address in Cminor *)
+      Cminor.eval_expr g sp locenv m (Eload AST.Mint32 nme_t) v_t  -> (* v_t is the value at address in CMinor *)
+      transl_value v v_t ->
+      is_copy_in le lprm lv_t -> 
+      is_copy_in (E_Name astnum nme::le) (prm::lprm) (addr_t::lv_t)
+  | Is_copy_in_Out: ∀ astnum le prm lprm nme v v_t nme_t lv_t,
+      parameter_mode prm = Out ->
+      transl_name stbl CE nme = OK nme_t -> (* nme_t is the expresion denoting the address where nme is stored in Cminor *)
+      eval_expr stbl s (E_Name astnum nme) (Normal v) -> (* addr is the evaluated variable *)
+      Cminor.eval_expr g sp locenv m (Eload AST.Mint32 nme_t) v_t  -> (* v_t is the value at address addr *)
+      transl_value v v_t -> (* This is not needed since Out variables wont be read before being written *)
+      is_copy_in le lprm lv_t -> 
+      is_copy_in (E_Name astnum nme::le) (prm::lprm) (v_t::lv_t).
+
+End is_copy.
+
+Lemma transl_copy_in_OK :
+  forall stbl s (*n*) prms args f fr fr',
+    copy_in stbl s fr prms args fr'
+    -> fr' = Normal f
+     -> forall CE g sp locenv m bl lv,
+         match_env stbl s CE sp locenv g m
+         -> transl_paramexprlist stbl CE args prms = OK bl
+         -> eval_exprlist g sp locenv m bl lv
+         -> is_copy_in stbl CE g sp locenv m s args prms lv.
+(* + matching vargs <-> bl *)
+Proof.
+  !!(intros until 1).
+(*   unfold transl_paramexprlist. *)
+  !induction h_copy_in_fr_fr'; !intros;try (discriminate);cbn in *.
+  - !inversion h_trans_prmexprl.
+    !inversion h_eval_exprlist.
+    constructor.
+  - rewrite heq in h_trans_prmexprl.
+    !destruct (transl_expr st CE e) !eqn:?; try discriminate;cbn in *.
+    !destruct (transl_paramexprlist st CE le lparam) !eqn:?; try discriminate;cbn in *.
+    !invclear h_trans_prmexprl.
+    up_type.
+    !inversion h_eval_exprlist.
+    econstructor;eauto.
+    !destruct (transl_expr_ok _ _ _ _ heq_tr_expr_e _ _ _ _ _ _ h_eval_expr_e_e_v h_match_env). 
+    !destruct h_and.
+    erewrite det_eval_expr with (v:=e_t_v) (v' := x);eauto.
+  - rewrite heq in h_trans_prmexprl.
+    !destruct (transl_expr st CE e) !eqn:?; try discriminate;cbn in *.
+    !destruct (transl_paramexprlist st CE le lparam) !eqn:?; try discriminate;cbn in *.
+    !invclear h_trans_prmexprl.
+    up_type.
+    !inversion h_eval_exprlist.
+    econstructor;eauto.
+    !destruct (transl_expr_ok _ _ _ _ heq_tr_expr_e _ _ _ _ _ _ h_eval_expr_e h_match_env). 
+    !destruct h_and.
+    erewrite det_eval_expr with (v:=e_t_v) (v' := x);eauto.
+  - rewrite heq in h_trans_prmexprl.
+    !destruct (transl_name st CE n) !eqn:?; try discriminate;cbn in *.    
+    !destruct (transl_paramexprlist st CE le lparam) !eqn:?; try discriminate;cbn in *.
+    !invclear h_trans_prmexprl.
+    up_type.
+    !inversion h_eval_exprlist.
+    econstructor 3;eauto 2. (* rec hyp used *)
+    + econstructor.
+      eassumption.
+    + econstructor;eauto.
+      generalize(h_match_env.(me_stack_complete));eauto.
+
+      xxxxxxxxxxxxxxx
 
 Lemma transl_copy_in_OK :
   forall stbl s (*n*) prms args f fr fr',
@@ -2455,30 +2567,144 @@ Lemma transl_copy_in_OK :
       -> fr' = Normal f
      -> forall CE g sp locenv m bl,
          match_env stbl s CE sp locenv g m
-         -> transl_exprlist stbl CE args = OK bl
+         -> transl_paramexprlist stbl CE args prms = OK bl
          (* vargs does not exists for Out parameters. TODO: restrict to In/In_Out parameters *)
          -> ∃ vargs, eval_exprlist g sp locenv m bl vargs.
 (* + matching vargs <-> bl *)
 Proof.
   !!(intros until 1).
-  !induction h_copy_in_fr_fr'; !intros;try discriminate;cbn in *.
-  - !inversion h_incr_order_fr.
-    subst.
+(*   unfold transl_paramexprlist. *)
+  !induction h_copy_in_fr_fr'; !intros;try (discriminate);cbn in *.
+  - !inversion h_trans_prmexprl.
     exists (@nil Values.val).
     constructor.
-  - !destruct (transl_expr st CE e) !eqn:?; try discriminate.
+  - rewrite heq in h_trans_prmexprl.
+    !destruct (transl_expr st CE e) !eqn:?; try discriminate.
      eapply transl_expr_ok in heq_tr_expr_e.
      + !! (destruct heq_tr_expr_e as [v_t [ ? ?]]).
-       !destruct (transl_exprlist st CE le) !eqn:?; try discriminate;cbn in *.
-       specialize (IHh_copy_in_fr_fr' heq_f'' _ _ _ _ _ _ h_match_env h_incr_order_fr0).
+       cbn in h_trans_prmexprl.
+       !destruct (transl_paramexprlist st CE le lparam) !eqn:?; try discriminate;cbn in *.
+       specialize (IHh_copy_in_fr_fr' heq_f'' _ _ _ _ _ _ h_match_env h_trans_prmexprl0).
        destruct IHh_copy_in_fr_fr' as [vargs IHh_copy_in_fr_fr'].
        up_type.
        exists (e_t_v :: vargs).
-       inversion h_incr_order_fr.
+       inversion h_trans_prmexprl.
        constructor;auto.
        eauto.
      + eassumption.
      + assumption.
+  - rewrite heq in h_trans_prmexprl.
+    !destruct (transl_expr st CE e) !eqn:?; try discriminate.
+     eapply transl_expr_ok in heq_tr_expr_e.
+     + !! (destruct heq_tr_expr_e as [v_t [ ? ?]]).
+       cbn in h_trans_prmexprl.
+       !destruct (transl_paramexprlist st CE le lparam) !eqn:?; try discriminate;cbn in *.
+       specialize (IHh_copy_in_fr_fr' heq_f'' _ _ _ _ _ _ h_match_env h_trans_prmexprl0).
+       destruct IHh_copy_in_fr_fr' as [vargs IHh_copy_in_fr_fr'].
+       up_type.
+       exists (e_t_v :: vargs).
+       inversion h_trans_prmexprl.
+       constructor;auto.
+       eauto.
+     + eassumption.
+     + assumption.   
+  - rewrite heq in h_trans_prmexprl.
+    !destruct (transl_name st CE n) !eqn:?; try discriminate;cbn in *.    
+    !destruct (transl_paramexprlist st CE le lparam) !eqn:?; try discriminate;cbn in *.
+    !invclear h_trans_prmexprl. 
+    specialize (IHh_copy_in_fr_fr' heq_f'' _ _ _ _ _ _ h_match_env h_trans_prmexprl0).
+    destruct IHh_copy_in_fr_fr' as [vargs IHh_copy_in_fr_fr'].
+    up_type.
+    !assert (exists n_t_v, transl_value v n_t_v ∧ Cminor.eval_expr g sp locenv m n_t n_t_v).
+    {  assert (h_ex_typ:exists (typ_nme:type) cm_typ_nme,
+                  (type_of_name st n =: typ_nme)
+                  ∧ (transl_type st typ_nme =: cm_typ_nme)
+                  ∧ (make_load n_t cm_typ_nme =: n_t)).
+       { admit. (* well formedness/typedness *) }  
+       decompose [ex and] h_ex_typ.
+       eapply (h_match_env.(me_stack_match));eauto. }
+    decomp h_ex.
+    exists (n_t_v::vargs);constructor;auto.
+  - rewrite heq in h_trans_prmexprl.
+    !destruct (transl_name st CE n) !eqn:?; try discriminate;cbn in *.    
+    !destruct (transl_paramexprlist st CE le lparam) !eqn:?; try discriminate;cbn in *.
+    !invclear h_trans_prmexprl. 
+    specialize (IHh_copy_in_fr_fr' heq_f'' _ _ _ _ _ _ h_match_env h_trans_prmexprl0).
+    destruct IHh_copy_in_fr_fr' as [vargs IHh_copy_in_fr_fr'].
+    up_type.
+    !assert (exists n_t_v, transl_value (Int v) n_t_v ∧ Cminor.eval_expr g sp locenv m n_t n_t_v).
+    {  assert (h_ex_typ:exists (typ_nme:type) cm_typ_nme,
+                  (type_of_name st n =: typ_nme)
+                  ∧ (transl_type st typ_nme =: cm_typ_nme)
+                  ∧ (make_load n_t cm_typ_nme =: n_t)).
+       { (* useful?: (h:stbl_var_types_ok st). consequence of invariant_compile CE *)
+         admit. (* well formedness/typedness *) }  
+       decompose [ex and] h_ex_typ.
+       eapply (h_match_env.(me_stack_match));eauto. }
+    decomp h_ex.
+    exists (n_t_v::vargs);constructor;auto.
+  - rewrite heq in h_trans_prmexprl.
+    !destruct (transl_name st CE n) !eqn:?; try discriminate;cbn in *.    
+    !destruct (transl_paramexprlist st CE le lparam) !eqn:?; try discriminate;cbn in *.
+    !invclear h_trans_prmexprl. 
+    specialize (IHh_copy_in_fr_fr' heq_f'' _ _ _ _ _ _ h_match_env h_trans_prmexprl0).
+    destruct IHh_copy_in_fr_fr' as [vargs IHh_copy_in_fr_fr'].
+    up_type.
+
+    !assert (exists n_t_v,Cminor.eval_expr g sp locenv m n_t n_t_v).
+    {  assert (h_ex_typ:exists (typ_nme:type) cm_typ_nme,
+                  (type_of_name st n =: typ_nme)
+                  ∧ (transl_type st typ_nme =: cm_typ_nme)
+                  ∧ (make_load n_t cm_typ_nme =: n_t)).
+       {
+         admit. (* well formedness/typedness *) }  
+       decompose [ex and] h_ex_typ.
+       eapply (h_match_env.(me_stack_match));eauto. }
+    decomp h_ex.
+    exists (n_t_v::vargs);constructor;auto.
+  -
+
+
+
+    
+
+    unfold stack_match in h_stk_mtch_s_m.
+    specialize (h_stk_mtch_s_m n v n_t).
+    destruct (type_of_name st n) eqn:heq_typ_n;cbn in h_stk_mtch_s_m.
+    + destruct (transl_type st t) eqn:heq_tr_typ_t.
+      * destruct (make_load n_t t0) eqn:heq_mkload_t0.
+        specialize (h_stk_mtch_s_m  e t t0 h_eval_name_n_v eq_refl heq_transl_name heq_tr_typ_t heq_mkload_t0) .
+        !! destruct h_stk_mtch_s_m as [v_t [? ?]].
+        !destruct (transl_paramexprlist st CE le lparam) !eqn:?; try discriminate;cbn in *.
+        specialize (IHh_copy_in_fr_fr' heq_f'' _ _ _ _ _ _ h_match_env h_trans_prmexprl0).
+        destruct IHh_copy_in_fr_fr' as [vargs IHh_copy_in_fr_fr'].
+        up_type.
+        exists (e_v::vargs).
+        inversion h_trans_prmexprl.
+        subst bl.
+        constructor;auto.
+        eauto.
+      * eassumption.
+      * assumption.
+
+)
+
+
+
+     eapply transl_name_ok in heq_transl_name.
+     + !! (destruct heq_tr_expr_e as [v_t [ ? ?]]).
+       cbn in h_trans_prmexprl.
+       !destruct (transl_paramexprlist st CE le lparam) !eqn:?; try discriminate;cbn in *.
+       specialize (IHh_copy_in_fr_fr' heq_f'' _ _ _ _ _ _ h_match_env h_trans_prmexprl0).
+       destruct IHh_copy_in_fr_fr' as [vargs IHh_copy_in_fr_fr'].
+       up_type.
+       exists (e_t_v :: vargs).
+       inversion h_trans_prmexprl.
+       constructor;auto.
+       eauto.
+     + eassumption.
+     + assumption.
+
   - !destruct (transl_expr st CE e) !eqn:?; try discriminate;cbn in *.
      eapply transl_expr_ok in heq_tr_expr_e.
      + !! (destruct heq_tr_expr_e as [v_t [ ? ?]]).
@@ -2521,11 +2747,12 @@ Proof.
        eassumption.
      + assumption.
   (* Out parameter, the variable is not evaluated at all, and may be undefined, on the spark side. In any case the value pushed is Undefined. *)
-  - !destruct (transl_expr st CE (E_Name ast_num n)) !eqn:?; try discriminate;cbn in *.
+  - specialize (IHh_copy_in_fr_fr' heq_f'').
+    !destruct (transl_expr st CE (E_Name ast_num n)) !eqn:?; try discriminate;cbn in *.
 (*      eapply transl_expr_ok in heq_tr_expr. *)
 (*      + !! (destruct heq_tr_expr as [? [ ? ?]]). *)
        !destruct (transl_exprlist st CE le) !eqn:?; try discriminate;cbn in *.
-       specialize (IHh_copy_in_fr_fr' heq_f'' _ _ _ _ _ _ h_match_env h_incr_order_fr0).
+       specialize (IHh_copy_in_fr_fr' _ _ _ _ _ _ h_match_env h_incr_order_fr0).
        destruct IHh_copy_in_fr_fr' as [vargs IHh_copy_in_fr_fr'].
        up_type.
        exists (Values.Vundef :: vargs). (* No value exists fo Out parameters? *)
@@ -2963,38 +3190,6 @@ Proof.
     (* TODO: deal with lvl_p = 0. *)
 
 (* *************************** SCRATCH  ************************** *)
-        (* Property linking spark args expr list , spark args value
-           list , Cminor args expr list and Cminor args value list. We
-           need to talk a bout expressions because Out and InOut
-           parameters are translated into names (and not expressions)
-           in order to be able to have there cminor address. Once the
-           prelude of the function is executed, all variables are in
-           the stack as standard variables. *)
-
-        Inductive is_copy_in (stbl : symboltable) (CE : compilenv):
-          (el : list expression) -> list parameter_specification -> list value -> list Values.val -> Prop :=
-        | Is_copy_in_nil: is_copy_in nil nil nil
-        | Is_copy_in_In: ∀ prm lprm v lv v_t lv_t,
-            parameter_mode prm = In ->
-            transl_value v v_t ->
-            is_copy_in lprm lv lv_t -> 
-            is_copy_in (prm::lprm) (v :: lv) (v_t::lv_t)
-        | Is_copy_in_In_Out: ∀ prm lprm nme lv nme_t lv_t,
-            parameter_mode prm = In_Out ->
-            transl_name v v_t ->
-            is_copy_in lprm lv lv_t -> 
-            is_copy_in (prm::lprm) (Undefined :: lv) (v_t::lv_t)
-        | Is_copy_in_In_Out: ∀ prm lprm v lv v_t lv_t,
-            parameter_mode prm = Out ->
-            is_copy_in lprm lv lv_t -> 
-            is_copy_in (prm::lprm) (Undefined :: lv) (v_t::lv_t).
-
-        assert ((copy_in st s (newFrame n) (procedure_parameter_profile pb) args (Normal f))
-         -> transl_paramexprlist st CE args (procedure_parameter_profile pb) =: args_t
-         -> exists chain_addr sto,
-             eval_exprlist g (Values.Vptr spb ofs) locenv m
-                           (build_loads_ (Datatypes.length CE - 1 - lvl_p) :: args_t) (chain_addr::sto)
-             ∧ is_copy_in (procedure_parameter_profile pb) f sto).
 
 
 (* *************************** END SCRATCH ************************ *)
